move proofs

examples/heapsort/HeapsortProperties.v
@@ -10,4 +10,1506 @@ Require Import
 From Coq.Program Require Import Basics Wf.
 Import Nat.
 Import ListNotations.
+Require Import HeapsortHeader.
 Local Open Scope program_scope.
+
+Section BinaryTreeIndexing.
+
+  Lemma unfold_decode i :
+    decodeIdx i =
+    if Nat.eq_dec i 0 then [] else
+    if Nat.eq_dec (i mod 2) 1
+    then decodeIdx ((i - 1) / 2) ++ [Dir_left]
+    else decodeIdx ((i - 2) / 2) ++ [Dir_right].
+  Proof with lia || discriminate || eauto.
+    apply encode_inj. rewrite encode_decode.
+    destruct (Nat.eq_dec i 0) as [H_yes1 | H_no1]...
+    assert (claim1 := Nat.mod_bound_pos i 2).
+    destruct (Nat.eq_dec (i mod 2) 1) as [H_yes2 | H_no2];
+      [assert (claim2 := encode_decode ((i - 1) / 2)) | assert (claim2 := encode_decode ((i - 2) / 2))].
+    all: symmetry; revert claim2; unfold encodeIdx; intros H_eq;
+      rewrite fold_left_last; unfold dir_t_rect at 1;
+      rewrite H_eq; symmetry.
+    - apply positive_odd...
+    - apply positive_even...
+  Qed.
+
+  Lemma decode_nat n :
+    match decodeIdx n with
+    | [] => n = 0
+    | Dir_left :: l => encodeIdx l = n - 2 ^ (length (decodeIdx n)-1)
+    | Dir_right :: l => encodeIdx l = n - 2 ^ (length (decodeIdx n))
+    end.
+  Proof with auto.
+    destruct (decodeIdx n) eqn:E.
+    - apply (f_equal encodeIdx) in E;rewrite (encode_decode n) in E.
+      unfold encodeIdx in E; simpl in E...
+    - apply (f_equal encodeIdx) in E;rewrite (encode_decode n) in E;rewrite E.
+      rewrite (encode_unfold (d :: l)). destruct d;simpl;nia.
+  Qed.
+
+  Lemma encode_bound l n : length l = n -> 2^n -1 <= encodeIdx l < 2 ^ (S n) -1.
+  Proof.
+    revert n. induction l;intros.
+    - simpl in *. rewrite <- H. simpl. auto.
+    - simpl in *. destruct n;inversion H.
+      rewrite encode_unfold. destruct a.
+      + simpl. rewrite H1. apply IHl in H1. rewrite sub_0_r.
+        pose_exp2 n. lia.
+      + simpl. rewrite H1. apply IHl in H1.
+        pose_exp2 n. lia.
+  Qed.
+  
+  Lemma decode_ubound j n : j < 2 ^ n - 1 -> length (decodeIdx j) < n.
+  Proof.
+    intros. pose proof (lt_dec (length (decodeIdx j)) n) as Y.
+    destruct Y;auto.
+    assert (length (decodeIdx j) >= n) by nia.
+    remember (length (decodeIdx j)) as m.
+    symmetry in Heqm. apply encode_bound in Heqm.
+    rewrite encode_decode in Heqm.
+    assert (2 ^ n <= 2 ^ m) by now apply pow_le_mono_r.
+    nia.
+  Qed.
+
+  Lemma decode_lbound j n : 2 ^ n -1 <= j -> n <= length (decodeIdx j).
+  Proof.
+    intros. pose proof (lt_dec n (S (length (decodeIdx j)))) as Y.
+    destruct Y; try nia.
+    assert (S (length (decodeIdx j)) <= n) by nia.
+    remember (length (decodeIdx j)) as m.
+    symmetry in Heqm. apply encode_bound in Heqm.
+    rewrite encode_decode in Heqm.
+    assert (2 ^ S m <= 2 ^ n) by now apply pow_le_mono_r.
+    nia.
+  Qed.
+
+  Lemma encode_lt_eqlen d i j : length i = length j -> encodeIdx (d :: i) < encodeIdx (d :: j) -> encodeIdx i < encodeIdx j.
+  Proof.
+    intro H.
+    rewrite (encode_unfold (d :: i)).
+    rewrite (encode_unfold (d :: j)).
+    simpl length. rewrite H.
+    destruct d; lia.
+  Qed.
+
+  Lemma btidx_lt_complete i j : encodeIdx i < encodeIdx j -> btidx_lt i j.
+  Proof.
+    assert (length i < length j \/ length i = length j \/ length i > length j) by lia.
+    destruct H as [|[]].
+    - unfold btidx_lt. left. assumption.
+    - intros H1. right.
+      revert j H H1.
+      induction i as [|x i].
+      + intros. destruct j; simpl in H; try lia.
+      + intros. destruct j as [|y j]; simpl in H; try lia.
+        eapply succ_inj in H.
+        destruct x, y.
+        * econstructor. eapply IHi.
+          -- assumption.
+          -- eapply encode_lt_eqlen; eassumption.
+        * econstructor. assumption.
+        * exfalso.
+          rewrite (encode_unfold (Dir_right :: i)) in H1.
+          rewrite (encode_unfold (Dir_left :: j)) in H1.
+          simpl length in H1.
+          rewrite <- H in H1.
+          remember (length i) as n.
+          assert (2 ^ n - 1 <= encodeIdx i < 2 ^ S n - 1) by (eapply encode_bound; auto).
+          assert (2 ^ n - 1 <= encodeIdx j < 2 ^ S n - 1) by (eapply encode_bound; auto).
+          simpl pow in *. rewrite sub_0_r in H1. lia.
+        * econstructor. eapply IHi.
+          -- assumption.
+          -- eapply encode_lt_eqlen; eassumption.
+    - intros H'. exfalso.
+      remember (length i) as m.
+      remember (length j) as n.
+      assert (2 ^ m - 1 <= encodeIdx i < 2 ^ S m - 1) by (eapply encode_bound; auto).
+      assert (2 ^ n - 1 <= encodeIdx j < 2 ^ S n - 1) by (eapply encode_bound; auto).
+      assert (2 ^ S n <= 2 ^ m) by (eapply pow_le_mono_r; lia).
+      lia.
+  Qed.
+
+End BinaryTreeIndexing.
+
+Section BinaryTreeAccessories.
+
+  Context {A : Type}.
+
+  Lemma unfold_option_subtree ds t :
+    option_subtree ds t =
+    match ds with
+    | [] => Some t
+    | d :: ds' =>
+      match t with
+      | BT_nil => None
+      | BT_node x l r => option_subtree ds' (dir_t_rect (fun _ => bintree A) l r d)
+      end
+    end.
+  Proof. induction ds as [ | [ | ] ds IH]; eauto. Qed.
+
+  Lemma option_subtree_last ds d :
+    forall (root : bintree A),
+    option_subtree (ds ++ [d]) root =
+    match option_subtree ds root with
+    | None => None
+    | Some t => 
+      match t with
+      | BT_nil => None
+      | BT_node x l r => Some (dir_t_rect (fun _ => bintree A) l r d)
+      end
+    end.
+  Proof.
+    enough (claim1 : @option_subtree A (ds ++ [d]) = fold_right subtree_step (subtree_step d subtree_init) ds).
+    - rewrite claim1. clear claim1. unfold option_subtree. induction ds; destruct d; destruct root; eauto.
+    - unfold option_subtree at 1. rewrite <- rev_involutive with (l := ds ++ [d]) at 1.
+      rewrite fold_left_rev_right, rev_unit. simpl. now rewrite <- fold_left_rev_right, rev_involutive.
+  Qed.
+
+  Lemma option_subtree_last' i (t : bintree A) :
+    match option_subtree i t with
+    | Some (BT_node x l r) =>
+      option_subtree (i ++ [Dir_left]) t = Some l /\
+      option_subtree (i ++ [Dir_right]) t = Some r
+    | _ => True
+    end.
+  Proof.
+    assert (H1 := option_subtree_last i Dir_left t).
+    assert (H2 := option_subtree_last i Dir_right t).
+    destruct (option_subtree i t) as [ [] |]; auto.
+  Qed.
+
+  (*
+  Inductive occurs (t : bintree A) : list dir_t -> bintree A -> Prop :=
+  | Occurs_0
+    : occurs t [] t
+  | Occurs_l ds x l r
+    (H_l : occurs t ds l)
+    : occurs t (Dir_left :: ds) (BT_node x l r)
+  | Occurs_r ds x l r
+    (H_r : occurs t ds r)
+    : occurs t (Dir_right :: ds) (BT_node x l r).
+
+  Local Hint Constructors occurs : core.
+
+  Lemma occurs_iff ds t root :
+    occurs t ds root <->
+    option_subtree ds root = Some t.
+  Proof with discriminate || eauto.
+    split. intros X; induction X... revert t root.
+    induction ds as [ | [ | ] ds IH]; simpl; intros t root H_eq.
+    { apply Some_inj in H_eq; subst... }
+    all: destruct root as [ | x l r]...
+  Qed.
+   *)
+
+  Lemma toListAux_fromListAux (xss : list (list A)) : complete_list 0 xss -> toListAux (fromListAux xss) = xss.
+  Proof.
+    remember (length xss) as l eqn: H.
+    revert xss H.
+    induction l using Wf_nat.lt_wf_ind.
+    - rename H into IH. intros xss H1 H2.
+      destruct xss as [|xs xss]; auto.
+      destruct xs as [|x xs]; simpl in H2.
+      + destruct H2; destruct H; lia.
+      + destruct H2; destruct H; assert (xs = [])
+          by (eapply length_zero_iff_nil; lia);
+        subst; try reflexivity.
+        rewrite unfold_fromListAux.
+        simpl.
+        erewrite IH with (xss := splitLListLeft 0 xss); try reflexivity.
+        erewrite IH with (xss := splitLListRight 0 xss); try reflexivity.
+        rewrite zip_split by assumption.
+        reflexivity.
+        * assert (length (splitLListRight 0 xss) <= length xss)
+            by eapply splitLListRight_length.
+          simpl. lia.
+        * eapply complete_splitLListRight; assumption.
+        * rewrite splitLListLeft_length. simpl. lia.
+        * eapply complete_splitLListLeft; assumption.
+  Qed.
+
+  Lemma toList_fromList (xs : list A) : toList (fromList xs) = xs.
+  Proof.
+    unfold fromList, toList.
+    rewrite toListAux_fromListAux by eapply complete_toLList.
+    eapply concat_toLList.
+  Qed.
+
+  Lemma toList_length (t : bintree A) : length (toList t) = btsize t.
+  Proof.
+    unfold toList. induction t.
+    - simpl. auto.
+    - simpl. rewrite <- IHt1. rewrite <- IHt2.
+      apply f_equal. remember (toListAux t1) as xss1. remember (toListAux t2) as xss2.
+      clear IHt1 IHt2 Heqxss1 Heqxss2.
+      revert xss2. induction xss1.
+      + simpl. auto.
+      + intros. destruct xss2.
+        * simpl. nia.
+        * simpl. rewrite app_length. rewrite IHxss1.
+          do 3 rewrite app_length. nia.
+  Qed.
+
+  Lemma toList_step (t : bintree A) : btsize t >= 1 -> match t with
+                                       | BT_nil => False
+                                       | BT_node x _ _ => toList t = x :: tail (toList t)
+                                       end.
+  Proof.
+    intros.
+    destruct t; simpl in H; try lia.
+    reflexivity.
+  Qed.
+
+  Lemma toList_permutation (x : A) l r : Permutation (toList (BT_node x l r)) ([x] ++ (toList l) ++ (toList r)).
+  Proof.
+    unfold toList. simpl.
+    rewrite zipLList_permutation.
+    reflexivity.
+  Qed.
+
+  Lemma toList_btin (x : A) t : In x (toList t) -> btin x t.
+  Proof.
+    induction t.
+    - simpl. contradiction.
+    - simpl.
+      intros.
+      destruct H.
+      + subst. econstructor.
+      + assert (In x (toList t1) \/ In x (toList t2))
+          by (apply In_zipLList; assumption).
+        destruct H0.
+        * eapply btin_left.
+          eapply IHt1.
+          assumption.
+        * eapply btin_right.
+          eapply IHt2.
+          assumption.
+  Qed.
+
+  Lemma btpartial_fromListAux (xss : list (list A)) (y : A) :
+    complete_list 0 xss ->
+    btpartial (fromList (concat xss ++ [y])) (fromListAux xss).
+  Proof.
+    unfold fromList.
+    remember (length xss) as n.
+    revert xss Heqn.
+    induction n as [n IH] using Wf_nat.lt_wf_ind. intros.
+    destruct n.
+    - destruct xss; try discriminate.
+      vm_compute. econstructor.
+    - destruct xss as [| xs xss ]; try discriminate.
+      rewrite unfold_toLList.
+      replace (null _) with false by dec_list.
+      simpl in H, Heqn.
+      destruct H as [[H1 H2] | [H1 H2]]; try lia.
+      destruct xs as [| x []]; try discriminate. simpl.
+      rewrite unfold_fromListAux.
+      rewrite (unfold_fromListAux ([x] :: xss)).
+      econstructor.
+      + destruct (splitLListLeft_toLList_concat 0 xss y H2).
+        * rewrite H.
+          eapply (IH n).
+          -- lia.
+          -- rewrite splitLListLeft_length. lia.
+          -- eapply complete_splitLListLeft. assumption.
+        * rewrite H. eapply btpartial_refl.
+      + destruct (splitLListRight_toLList_concat 0 xss y H2).
+        * rewrite H.
+          eapply IH.
+          2: reflexivity.
+          -- pose proof (splitLListRight_length 0 xss). lia.
+          -- eapply complete_splitLListRight. assumption.
+        * rewrite H.
+          eapply btpartial_refl.
+  Qed.
+
+  Lemma btpartial_fromList (xs : list A) y :
+    btpartial (fromList (xs ++ [y])) (fromList xs).
+  Proof.
+    unfold fromList.
+    remember (toLList 0 xs) as xss.
+    assert (xs = concat xss) by (subst; rewrite concat_toLList; reflexivity).
+    rewrite H.
+    eapply btpartial_fromListAux.
+    subst.
+    eapply complete_toLList.
+  Qed.
+
+End BinaryTreeAccessories.
+
+Section CompleteBinaryTree.
+
+  Context {A : Type}.
+
+  Lemma perfect'2complete' {n} (t : bintree A)
+    (H_perfect : perfect' t n)
+    : complete' t n.
+  Proof.
+    induction H_perfect as [ | n x l r H_l IH_l H_r IH_r].
+    - exact (complete_nil).
+    - exact (complete_node_perfect_complete x l r H_l IH_r).
+  Qed.
+
+  Lemma complete_ind_ranked (P : bintree A -> nat -> Prop) :
+    P BT_nil 0 ->
+    (forall x l r n_l n_r, (n_r = n_l \/ S n_r = n_l) ->
+                      complete' l n_l -> complete' r n_r ->
+                      P l n_l -> P r n_r ->
+                      P (BT_node x l r) (S n_l)) ->
+    forall t n, complete' t n -> P t n.
+  Proof.
+    intros H_base H_ind t n H_complete.
+    revert t H_complete.
+    induction n using Wf_nat.lt_wf_ind.
+    intros t H_complete.
+    destruct H_complete as [| n x l r H_l H_r | n x l r H_l H_r ].
+    - exact H_base.
+    - assert (H_l' : complete' l n) by (eapply perfect'2complete'; assumption).
+      eapply H_ind.
+      + left. reflexivity.
+      + assumption.
+      + assumption.
+      + eapply H; try lia; assumption.
+      + eapply H; try lia; assumption.
+    - assert (H_r' : complete' r n) by (eapply perfect'2complete'; assumption).
+      eapply H_ind.
+      + right. reflexivity.
+      + assumption.
+      + assumption.
+      + eapply H; try lia; assumption.
+      + eapply H; try lia; assumption.
+  Qed.
+
+  Lemma perf_size (t : bintree A) n :
+    perfect' t n ->
+    btsize t = 2 ^ n -1.
+  Proof.
+    intros. induction H;auto.
+    simpl. rewrite IHperfect'1. rewrite IHperfect'2.
+    pose_exp2 n. lia.
+  Qed.
+
+  Lemma comp_size (t : bintree A) n :
+    complete' t (S n) ->
+    2 ^ n <= btsize t <= 2 ^ (S n) - 1.
+  Proof.
+    revert t. induction n;intros.
+    - inversion H;subst. simpl. inversion H_l;subst. inversion H_r;subst. simpl. auto.
+    - inversion H;subst.
+      + apply perf_size in H_l. simpl. rewrite H_l.
+        rewrite <- add_succ_l. pose_exp2 n.
+        replace (S (2 ^ n -1)) with (2 ^ n) by nia.
+        assert (btsize r <= 2 ^ S n - 1).
+        * clear IHn H0 H_l H l x.
+          admit. (*
+          induction H_r using complete_ind_ranked. simpl.
+          ** pose_exp2 n. lia.
+          ** destruct H;subst.
+             *** simpl in *. pose_exp2 n_l. lia.
+             *** simpl in *. pose_exp2 n_r. lia.
+             *)
+        * simpl in *. nia.
+      + apply perf_size in H_r. simpl. rewrite H_r.
+        rewrite <- add_succ_r.
+        apply IHn in H_l.
+        pose_exp2 n.
+        replace (S (2 ^ n - 1)) with (2 ^ n) by nia.
+        simpl in *. nia.
+  Admitted.
+
+(*
+  Ltac destruct_perfect t x l r :=
+    match goal with
+    | [ H : perfect_bintree ?n |- _ ] => 
+      constr_eq H t;
+      let n0 := fresh "n" in
+      let n1 := fresh "n" in
+      let Heq := fresh "Heq" in
+      remember n as n0 eqn: Heq in t;
+      destruct H as [|n1 x l r];
+      inversion Heq;
+      subst;
+      clear Heq
+    end.
+
+  Ltac destruct_complete t x l r :=
+    match goal with
+    | [ H : complete_bintree ?n |- _ ] =>
+      constr_eq H t;
+      let n0 := fresh "n" in
+      let n1 := fresh "n" in
+      let Heq := fresh "Heq" in
+      remember n as n0 eqn: Heq in t;
+      destruct H as [| n1 x l r | n1 x l r];
+      inversion Heq;
+      subst;
+      clear Heq
+    end.
+
+  Fixpoint delete_last_perfect {n} (t : perfect_bintree (S (S n))) : complete_bintree (S (S n)).
+  Proof.
+    destruct_perfect t x l r.
+    destruct n.
+    - assert (l' : complete_bintree 1)
+        by exact (perfect2complete l).
+      exact (complete_node_complete_perfect x l' perfect_nil).
+    - assert (r' : complete_bintree (S (S n)))
+        by exact (delete_last_perfect _ r).
+      exact (complete_node_perfect_complete x l r').
+  Defined.
+
+  Fixpoint delete_last_complete {n} (t : complete_bintree (S n)) : complete_bintree (S n) + perfect_bintree n.
+  Proof.
+    destruct_complete t x l r.
+    - destruct n.
+      + right. econstructor.
+      + left.
+        assert (r' : complete_bintree (S n) + perfect_bintree n) by exact (delete_last_complete _ r).
+        destruct r' as [r'|r'].
+        * exact (complete_node_perfect_complete x l r').
+        * exact (complete_node_complete_perfect x (perfect2complete l) r').
+    - assert (l' : complete_bintree (S n1) + perfect_bintree n1) by exact (delete_last_complete _ l).
+      destruct l' as [l'|l'].
+      + left. exact (complete_node_complete_perfect x l' r).
+      + right. exact (perfect_node x l' r).
+  Defined.
+ *)
+  Definition last_index (t : bintree A) := decode (btsize t - 1).
+
+  Lemma perfect'_rank (t : bintree A) n
+    (H_perfect : perfect' t n)
+    : rank t = n.
+  Proof. induction H_perfect; simpl; lia. Qed.
+
+  Lemma complete'_rank (t : bintree A) n
+    (H_complete : complete' t n)
+    : rank t = n.
+  Proof. induction H_complete. 2: apply perfect'_rank in H_l. 3: apply perfect'_rank in H_r. all: simpl; lia. Qed.
+
+  Lemma last_btidx_nil : last_btidx (BT_nil : bintree A) = [].
+  Proof. reflexivity. Qed.
+
+  Lemma btidx_lt_mono i j x y :
+    btidx_lt i j -> btidx_lt (i ++ [x]) (j ++ [y]).
+  Proof.
+    intros H.
+    destruct H.
+    - left. unfold lt_ltlen in *.
+      rewrite 2 app_length. simpl. lia.
+    - right.
+      induction H.
+      + simpl. econstructor. rewrite 2 app_length. simpl. lia.
+      + simpl. econstructor. assumption.
+  Qed.
+
+  Lemma last_btidx_half (t : bintree A) j d :
+    btidx_lt (removelast (last_btidx t)) j ->
+    btidx_lt (last_btidx t) (j ++ [d]).
+  Proof.
+    intros H.
+    remember (last_btidx t) as i; clear Heqi.
+    assert (Hnil : i = [] \/ i <> []) by (destruct i; [ left; reflexivity | right; congruence ]).
+    destruct Hnil.
+    - subst i. left. unfold lt_ltlen.
+      rewrite app_length.
+      simpl. lia.
+    - rewrite (app_removelast_last Dir_left H0).
+      eapply btidx_lt_mono.
+      assumption.
+  Qed.
+
+  Lemma last_btidx_perfect_complete (x : A) l r n :
+    n > 0 ->
+    perfect' l n ->
+    complete' r n ->
+    last_btidx (BT_node x l r) = Dir_right :: last_btidx r.
+  Proof.
+    intros. unfold last_btidx. simpl. rewrite sub_0_r.
+    apply encode_inj. rewrite (encode_decode _).
+    rewrite encode_unfold. rewrite (encode_decode _). simpl length.
+    rewrite (perf_size _ _ H0).
+    destruct n.
+    - inversion H.
+    - apply comp_size in H1. destruct H1. pose proof H1 as R.
+      eapply sub_le_mono_r with (p:=1) in H1.
+      eapply sub_le_mono_r with (p:=1) in H2.
+      apply decode_lbound in H1.
+      assert (btsize r -1 < 2 ^ S n -1).
+      + apply Lt.le_lt_n_Sm in H2.  rewrite <- sub_succ_l in H2.
+        2: { simpl. pose_exp2 n. lia. }
+        replace (S (2 ^ S n - 1) - 1) with (2 ^ S n - 1) in H2 by nia. auto.
+      + apply decode_ubound in H3. assert (length (decode (btsize r - 1)) = n) by nia.
+        rewrite H4. simpl. pose_exp2 n. lia.
+  Qed.
+    
+  Lemma last_btidx_complete_perfect (x : A) l r n :
+    complete' l (S n) ->
+    perfect' r n ->
+    last_btidx (BT_node x l r) = Dir_left :: last_btidx l.
+  Proof.
+    intros. unfold last_btidx. simpl. rewrite sub_0_r.
+    apply encode_inj. rewrite (encode_decode _).
+    rewrite encode_unfold. rewrite (encode_decode _). simpl length.
+    rewrite (perf_size _ _ H0).
+    apply comp_size in H. destruct H. pose proof H1 as R. pose proof H as T.
+    apply sub_le_mono_r with (p:=1) in H.
+    apply sub_le_mono_r with (p:=1) in H1.
+    apply decode_lbound in H.
+    pose_exp2 n.
+    assert (2 ^ S n >= 2) by (simpl;nia).
+    assert (btsize l - 1 < 2 ^ S n - 1) by nia.
+    apply decode_ubound in H4. assert (length (decode (btsize l -1)) = n) by nia.
+    rewrite H5. simpl. rewrite sub_0_r. nia.
+  Qed.
+
+  Lemma complete'_last_btidx_length (t : bintree A) n :
+    complete' t n ->
+    length (last_btidx t) = n - 1.
+  Proof.
+    intros H.
+    induction H as [| n x l r H_l H_r | n x l r H_l H_r].
+    - reflexivity.
+    - destruct n.
+      + inversion H_l.
+        inversion H_r.
+        subst.
+        reflexivity.
+      + erewrite last_btidx_perfect_complete with (n := S n)
+          by (try lia; eassumption).
+        simpl.
+        lia.
+    - erewrite last_btidx_complete_perfect
+        by eassumption.
+      simpl.
+      lia.
+  Qed.
+
+  Lemma subtree_outrange_ltlen (t : bintree A) :
+    complete t ->
+    forall j, lt_ltlen (last_btidx t) j ->
+         option_subtree j t = Some BT_nil \/ option_subtree j t = None.
+  Proof with first [ lia | eassumption | eapply perfect'2complete'; eassumption | idtac ].
+    unfold lt_ltlen.
+    intros [n H] j Hj.
+    revert t H j Hj.
+    induction n using Wf_nat.lt_wf_ind; rename H into IH.
+    intros t H j Hj.
+    destruct H.
+    - destruct j; auto.
+    - destruct n.
+      { inversion H_l.
+        inversion H.
+        subst.
+        unfold last_btidx in Hj; rewrite unfold_decode in Hj; simpl in Hj.
+        destruct j; simpl in Hj; try lia.
+        destruct j as [| d' j].
+        - left. destruct d; reflexivity.
+        - right. destruct d; reflexivity.
+      }
+      erewrite last_btidx_perfect_complete with (n := S n) in Hj...
+      destruct j as [|[] j]; simpl in Hj...
+      + rewrite unfold_option_subtree; simpl.
+        erewrite complete'_last_btidx_length in Hj...
+        eapply (IH (S n))...
+        erewrite complete'_last_btidx_length...
+        lia.
+      + rewrite unfold_option_subtree; simpl.
+        eapply (IH (S n))...
+    - erewrite last_btidx_complete_perfect in Hj...
+      destruct j as [|[] j]; simpl in Hj...
+      + rewrite unfold_option_subtree; simpl.
+        eapply (IH (S n))...
+      + rewrite unfold_option_subtree; simpl.
+        erewrite complete'_last_btidx_length in Hj...
+        eapply (IH n)...
+        erewrite complete'_last_btidx_length...
+        lia.
+  Qed.
+
+  (* It's possible to prove option_subtree j t = Some BT_nil *)
+  Lemma subtree_outrange_eqlen (t : bintree A) :
+    complete t ->
+    forall j, lt_eqlen (last_btidx t) j ->
+         option_subtree j t = Some BT_nil \/ option_subtree j t = None.
+  Proof with first [ lia | eassumption | eapply perfect'2complete'; eassumption | idtac ].
+    intros [n H] j Hj.
+    revert t H j Hj.
+    induction n using Wf_nat.lt_wf_ind; rename H into IH.
+    intros t H j Hj.
+    destruct H.
+    - rewrite last_btidx_nil in Hj.
+      inversion Hj.
+    - destruct n.
+      { inversion H_l.
+        inversion H.
+        subst.
+        unfold last_btidx in Hj; rewrite unfold_decode in Hj; simpl in Hj.
+        inversion Hj.
+      }
+      erewrite last_btidx_perfect_complete with (n := S n) in Hj...
+      inversion Hj; subst.
+      rewrite unfold_option_subtree; simpl.
+      eapply (IH (S n))...
+    - erewrite last_btidx_complete_perfect in Hj...
+      inversion Hj; subst.
+      + rewrite unfold_option_subtree; simpl.
+        destruct n.
+        { inversion H_r.
+          inversion H.
+          inversion H_l.
+          inversion H_r0.
+          subst.
+          destruct j0; try discriminate.
+          auto.
+        }
+        eapply subtree_outrange_ltlen.
+        * eexists...
+        * unfold lt_ltlen.
+          rewrite <- H1.
+          erewrite 2 complete'_last_btidx_length...
+          lia.
+      + rewrite unfold_option_subtree; simpl.
+        eapply (IH (S n))...
+  Qed.
+
+  Lemma subtree_outrange (t : bintree A) :
+    complete t ->
+    forall j, btidx_lt (last_btidx t) j ->
+         option_subtree j t = Some BT_nil \/ option_subtree j t = None.
+  Proof.
+    intros H j Hj.
+    destruct Hj.
+    - eapply subtree_outrange_ltlen; assumption.
+    - eapply subtree_outrange_eqlen; assumption.
+  Qed.
+
+  Lemma subtree_leaf (t : bintree A) :
+    complete t ->
+    forall j, btidx_lt (removelast (last_btidx t)) j ->
+         match option_subtree j t with
+         | Some t' => leaf t'
+         | None => True
+         end.
+  Proof.
+    intros H j Hj.
+    assert (H1 := option_subtree_last' j t).
+    assert (Hlt : forall d, btidx_lt (last_btidx t) (j ++ [d])) by (intros; eapply last_btidx_half; eassumption).
+    destruct (option_subtree j t) as [[]|].
+    - auto.
+    - destruct H1 as [Hl Hr]. split.
+      + destruct (subtree_outrange t H _ (Hlt Dir_left)) as [H2|H2];
+          rewrite H2 in Hl; inversion Hl.
+        reflexivity.
+      + destruct (subtree_outrange t H _ (Hlt Dir_right)) as [H2|H2];
+          rewrite H2 in Hr; inversion Hr.
+        reflexivity.
+    - auto.
+  Qed.
+
+  (*
+  Lemma subtree_nat_outrange j (t : bintree A) :
+    complete t -> j >= btsize t ->
+    subtree_nat t j = Some BT_nil \/ subtree_nat t j = None.
+  Proof.
+    intros.
+    destruct H.
+    destruct t eqn:E.
+    - unfold subtree_nat.
+      destruct (decode j);auto.
+    - assert (j > btsize (BT_node x0 b1 b2) - 1).
+      + pose proof (sub_le_mono_r _ _ 1 H0) as T.
+        simpl in H0. assert (j > j - 1) by nia. nia.
+      + rewrite <- (encode_decode j) in H1.
+        rewrite <- (encode_decode (btsize (BT_node _ _ _) -1)) in H1.
+        apply nat_btidx_iff in H1. destruct H1.
+        * eapply subtree_outrange_ltlen;eauto. exists x;auto.
+        * eapply subtree_outrange_eqlen;eauto. exists x;auto.
+  Qed.
+   *)
+
+  Lemma encode_removelast j : encode (removelast j) = (encode j + 1) / 2 - 1.
+  Proof.
+    assert (j = [] \/ j <> [])
+      by (destruct j; [ left; reflexivity | right; congruence]).
+    destruct H.
+    - subst j. reflexivity.
+    - rewrite (app_removelast_last Dir_left H) at 2.
+      rewrite encode_last.
+      remember (encode (removelast j)) as n.
+      destruct (last j Dir_left).
+      + replace (2 * n + 1 + 1) with ((n + 1) * 2) by lia.
+        rewrite div_mul by lia.
+        lia.
+      + replace (2 * n + 2 + 1) with (3 + n * 2) by lia.
+        rewrite div_add by lia.
+        simpl. lia.
+  Qed.
+
+  Lemma subtree_nat_leaf (t : bintree A) :
+    complete t ->
+    forall j, j > btsize t / 2 ->
+         match subtree_nat t (j - 1) with
+         | None => True
+         | Some t' => leaf t'
+         end.
+  Proof.
+    intros.
+    assert (Hs : btsize t <= 1 \/ btsize t > 1) by lia.
+    destruct Hs.
+    - unfold subtree_nat.
+      destruct t as [|x [] []]; simpl in H1; try lia.
+      + destruct (decode (j - 1)); simpl; auto.
+      + destruct (decode (j - 1)) as [| [] [] ]; simpl; auto.
+    - eapply subtree_leaf; try assumption.
+      unfold last_btidx.
+      eapply btidx_lt_complete.
+      rewrite encode_removelast.
+      rewrite 2 encode_decode.
+      rewrite sub_add by lia.
+      assert (1 <= btsize t / 2)
+        by (eapply (div_le_mono 2 _ 2); lia).
+      lia.
+  Qed.
+
+  Lemma perfect_fromListAux (xss : list (list A)) :
+    perfect_list 0 xss -> perfect' (fromListAux xss) (length xss).
+  Proof.
+    remember (length xss) as n.
+    revert xss Heqn.
+    induction n; intros.
+    - destruct xss; try discriminate.
+      rewrite unfold_fromListAux.
+      constructor.
+    - destruct xss as [|[|x xs] xss]; simpl in *; destruct H; try discriminate.
+      rewrite unfold_fromListAux.
+      econstructor.
+      + eapply IHn.
+        * rewrite splitLListLeft_length.
+          lia.
+        * eapply perfect_splitLListLeft. assumption.
+      + eapply IHn.
+        * rewrite splitLListRight_length' by assumption.
+          lia.
+        * eapply perfect_splitLListRight. assumption.
+  Qed.
+
+  Lemma complete_fromListAux (xss : list (list A)) :
+    complete_list 0 xss -> complete' (fromListAux xss) (length xss).
+  Proof.
+    remember (length xss) as n.
+    revert xss Heqn.
+    induction n using Wf_nat.lt_wf_ind. intros.
+    destruct n.
+    - destruct xss; try discriminate.
+      rewrite unfold_fromListAux.
+      econstructor.
+    - destruct xss as [|[|x xs] xss]; simpl in *; try discriminate; try lia.
+      eapply succ_inj in Heqn. subst.
+      rewrite unfold_fromListAux.
+      destruct H0 as [[]|[]].
+      + pose proof (complete_splitLList 0 xss H1).
+        remember (length xss) as n'.
+        remember (splitLListLeft 0 xss) as l.
+        remember (splitLListRight 0 xss) as r.
+        simpl in H2.
+        destruct H2 as [[Hl1 [Hl2 [Hr1 Hr2]]] | [Hl1 [Hl2 [Hr1 Hr2]]]].
+        * eapply complete_node_perfect_complete.
+          -- rewrite <- Hl2.
+             eapply perfect_fromListAux.
+             assumption.
+          -- eapply H; try lia; assumption.
+        * destruct Hr2 as [n'' []].
+          replace n' with (S n'') by lia.
+          eapply complete_node_complete_perfect.
+          -- eapply H; try lia; assumption.
+          -- rewrite <- H2.
+             eapply perfect_fromListAux.
+             assumption.
+      + subst. lia.
+  Qed.
+
+  Lemma complete_fromList (xs : list A) : complete (fromList xs).
+  Proof.
+    unfold complete, fromList.
+    remember (toLList 0 xs) as xss.
+    assert (H : complete_list 0 xss)
+      by (subst; eapply complete_toLList).
+    eexists. eapply complete_fromListAux. assumption.
+  Qed.
+
+  Lemma complete_toListAux_length n (t : bintree A) :
+    complete' t n -> length (toListAux t) = n.
+  Proof.
+    intros.
+    admit.
+    (*
+    induction H using complete_ind_ranked.
+    - reflexivity.
+    - simpl.
+      rewrite zipLList_length.
+      rewrite IHcomplete'1.
+      rewrite IHcomplete'2.
+      lia.
+     *)
+  Admitted.
+
+  Lemma perfect_toListAux_list (t : bintree A) :
+    perfect t -> perfect_list 0 (toListAux t).
+  Proof.
+    intros [n H].
+    induction H.
+    - simpl. auto.
+    - simpl. split; auto.
+      eapply perfect_zipLList; try assumption.
+      erewrite complete_toListAux_length by (eapply perfect'2complete'; eassumption).
+      erewrite complete_toListAux_length by (eapply perfect'2complete'; eassumption).
+      reflexivity.
+  Qed.
+
+  Lemma complete_toListAux_list (t : bintree A) :
+    complete t -> complete_list 0 (toListAux t).
+  Proof.
+    intros [n H].
+    induction H; simpl.
+    - auto.
+    - left. split; auto.
+      eapply complete_zipLList. left.
+      split; [|split].
+      + eapply perfect_toListAux_list. eexists. eassumption.
+      + assumption.
+      + erewrite complete_toListAux_length by (eapply perfect'2complete'; eassumption).
+        erewrite complete_toListAux_length by eassumption.
+        reflexivity.
+    - left. split; auto.
+      eapply complete_zipLList. right.
+      split; [|split].
+      + assumption.
+      + eapply perfect_toListAux_list. eexists. eassumption.
+      + erewrite complete_toListAux_length by eassumption.
+        erewrite complete_toListAux_length by (eapply perfect'2complete'; eassumption).
+        reflexivity.
+  Qed.
+
+  Lemma fromListAux_toListAux (t : bintree A) :
+    complete t -> fromListAux (toListAux t) = t.
+  Proof.
+    intros [n H].
+    revert t H.
+    induction n as [n IH] using Wf_nat.lt_wf_ind; intros.
+    inversion H; subst; clear H.
+    - reflexivity.
+    - rename n0 into n. simpl. rewrite unfold_fromListAux.
+      assert (H :
+                perfect_list 0 (toListAux l) /\
+                complete_list 0 (toListAux r) /\
+                length (toListAux l) = length (toListAux r)).
+      { split; [|split].
+        - eapply perfect_toListAux_list.
+          eexists; eassumption.
+        - eapply complete_toListAux_list.
+          eexists; eassumption.
+        - erewrite complete_toListAux_length by (eapply perfect'2complete'; eassumption).
+          erewrite complete_toListAux_length by eassumption.
+          reflexivity.
+      }
+      rewrite splitLeft_zip by auto.
+      rewrite splitRight_zip by auto.
+      erewrite (IH n).
+      erewrite (IH n).
+      reflexivity.
+      + lia.
+      + assumption.
+      + lia.
+      + eapply perfect'2complete'. assumption.
+    - rename n0 into n. simpl. rewrite unfold_fromListAux.
+      assert (H :
+                complete_list 0 (toListAux l) /\
+                perfect_list 0 (toListAux r) /\
+                length (toListAux l) = 1 + length (toListAux r)).
+      { split; [|split].
+        - eapply complete_toListAux_list.
+          eexists; eassumption.
+        - eapply perfect_toListAux_list.
+          eexists; eassumption.
+        - erewrite complete_toListAux_length by eassumption.
+          erewrite complete_toListAux_length by (eapply perfect'2complete'; eassumption).
+          reflexivity.
+      }
+      rewrite splitLeft_zip by auto.
+      rewrite splitRight_zip by auto.
+      erewrite (IH (S n)).
+      erewrite (IH n).
+      reflexivity.
+      + lia.
+      + eapply perfect'2complete'. assumption.
+      + lia.
+      + assumption.
+  Qed.
+
+  Lemma fromList_toList (t : bintree A) :
+    complete t -> fromList (toList t) = t.
+  Proof.
+    intros.
+    unfold toList.
+    unfold fromList.
+    rewrite toLList_concat by (eapply complete_toListAux_list; assumption).
+    eapply fromListAux_toListAux; assumption.
+  Qed.
+
+  Lemma subtree_index (tree : bintree A) t i :
+    complete tree
+    -> option_subtree i tree = Some t
+    -> forall n, lookup (toList t) n = lookup (toList tree) (n + (encode i) * 2 ^ (length (decode n))).
+  Admitted.
+
+  Lemma toList_subtree (tree : bintree A) i : lookup (toList tree) i =
+                                  match subtree_nat tree i with
+                                  | None => None
+                                  | Some t => option_root t
+                                  end.
+    Admitted.
+  
+  Theorem subtree_nat_Some_node (tree : bintree A) t i (t_nonempty : t <> BT_nil) :
+    subtree_nat tree i = Some t <->
+    match t with
+    | BT_nil => False
+    | BT_node x l r => HeapsortHeader.lookup (toList tree) i = Some x /\ subtree_nat tree (i * 2 + 1) = Some l /\ subtree_nat tree (i * 2 + 2) = Some r
+    end.
+  Admitted.
+
+  Theorem subtree_lookup (tree : bintree A) t i
+    (H_complete : complete tree)
+    (H_subtree : subtree_nat tree i = Some t)
+    : lookup (toList tree) i = option_root t.
+  Admitted.  
+
+  Corollary subtree_nat_range (tree : bintree A) t i
+    (H_complete : complete tree)
+    (H_subtree : subtree_nat tree i = Some t)
+    : i < btsize tree <-> t <> BT_nil.
+  Proof.
+    pose proof (subtree_lookup tree t i H_complete H_subtree) as claim1.
+    destruct t as [ | x l r]; [apply nth_error_None in claim1 | apply isSome_intro, nth_error_Some in claim1]; rewrite toList_length in claim1.
+    - split; [lia | contradiction].
+    - split; [discriminate | lia].
+  Qed.
+
+  Lemma option_subtree_swap (tree : bintree A) i j k :
+    k > i -> k > j ->
+    subtree_nat (fromList (swap (toList tree) i j)) k = subtree_nat tree k.
+  Admitted.
+  
+  Lemma btpartial_removelast (t : bintree A) :
+    complete t ->
+    btpartial t (fromList (removelast (toList t))).
+  Proof.
+    intros.
+    rewrite <- (fromList_toList t H) at 1.
+    destruct t.
+    - vm_compute. econstructor.
+    - remember (toList (BT_node x t1 t2)) as xs.
+      assert (xs <> [])
+        by (intro; subst; discriminate).
+      rewrite (app_removelast_last x H0) at 1.
+      eapply btpartial_fromList.
+  Qed.
+
+End CompleteBinaryTree.
+
+Section HeapProperty.
+
+  Context {A : Type}.
+  Variable R : A -> A -> Prop.
+
+  Lemma heap_erase_priority p t : heap_pr R p t -> heap R t.
+  Proof. intros. destruct H; econstructor; assumption. Qed.
+
+  Lemma heap_pr_if_heap (R_refl : forall x, R x x) t : t <> BT_nil -> heap R t -> exists p, heap_pr R p t.
+  Proof.
+    intros Ht Hₕ.
+    destruct Hₕ; try contradiction.
+    eexists.
+    econstructor; try assumption.
+    eapply R_refl.
+  Qed.
+
+  Lemma heap_at_0 t : heap_at R 0 t -> heap R t.
+  Proof.
+    Local Transparent decodeIdx.
+    unfold heap_at. simpl. tauto.
+  Qed.
+
+  Lemma heap_if_leaf t : leaf t -> heap R t.
+  Proof.
+    intro H. destruct t.
+    - econstructor.
+    - simpl in H. destruct H. subst. econstructor; econstructor.
+  Qed.
+
+  Lemma heap_at_leaves t : complete t -> forall j, j > btsize t / 2 -> heap_at R (j - 1) t.
+  Proof.
+    intros H j Hj. unfold heap_at.
+    assert (H1 := subtree_nat_leaf t H j Hj).
+    destruct (subtree_nat t (j-1)).
+    - eapply heap_if_leaf; assumption.
+    - auto.
+  Qed.
+
+  Lemma heap_btpartial t t' :
+    btpartial t t' -> heap R t -> heap R t'.
+  Proof.
+    intro H. induction H as [| x l r l' r' Hl IHl Hr IHr |].
+    - auto.
+    - intros Hₕ.
+      remember (BT_node x l r) eqn: E.
+      destruct Hₕ; try discriminate.
+      inversion E; subst; clear E.
+      econstructor.
+      + inversion Hl; subst; simpl in *; auto.
+      + inversion Hr; subst; simpl in *; auto.
+      + eapply IHl. assumption.
+      + eapply IHr. assumption.
+    - constructor.
+  Qed.
+
+  Lemma removelast_heap t :
+    complete t -> heap R t -> heap R (fromList (removelast (toList t))).
+  Proof.
+    intros. eapply heap_btpartial.
+    - eapply btpartial_removelast. assumption.
+    - assumption.
+  Qed.
+
+  Lemma heap_rel p t :
+    Transitive R ->
+    heap_pr R p t ->
+    forall x, btin x t -> R p x.
+  Proof.
+    intro T.
+    induction t.
+    - intros. inversion H0.
+    - intros.
+      remember (BT_node x t1 t2) as t eqn: E.
+      destruct H; try discriminate.
+      inversion E; subst; clear E.
+      remember (BT_node x t1 t2) as t eqn: E.
+      destruct H0; inversion E; subst; clear E.
+      + assumption.
+      + eapply IHt1.
+        * destruct heap_l; econstructor; try assumption.
+          transitivity x; assumption.
+        * assumption.
+      + eapply IHt2.
+        * destruct heap_r; econstructor; try assumption.
+          transitivity x; assumption.
+        * assumption.
+  Qed.
+
+  Lemma heap_head_last t x xs a :
+    Reflexive R ->
+    Transitive R ->
+    heap R t ->
+    toList t = x :: xs ->
+    R x (last (toList t) a).
+  Proof.
+    intros.
+    eapply heap_rel.
+    - assumption.
+    - instantiate (1 := t).
+      destruct H1; try discriminate.
+      unfold toList in H2.
+      simpl in H2. inversion H2; subst.
+      econstructor; try assumption.
+      eapply H.
+    - eapply toList_btin.
+      eapply In_last.
+      intro. rewrite H3 in H2. discriminate.
+  Qed.
+
+End HeapProperty.
+
+Section BinaryTreeZipper.
+
+  Context {A : Type}.
+
+  Lemma recover_focus (g : btctx A) t i :
+    let '(g', t') := focus g t i in
+    recover_bintree g t = recover_bintree g' t'.
+  Proof.
+    revert g t.
+    induction i.
+    - intros g t. destruct t; reflexivity.
+    - intros g t.
+      destruct t, a; try reflexivity; simpl.
+      + pose proof (IHi (btctx_left x t2 g) t1).
+        destruct (focus (btctx_left x t2 g) t1 i) as [g' t'].
+        auto.
+      + pose proof (IHi (btctx_right x t1 g) t2).
+        destruct (focus (btctx_right x t2 g) t2 i) as [g' t'].
+        auto.
+  Qed.
+
+  Lemma focus_recover (tree : bintree A) t i j:
+    let '(g', _) := focus btctx_top tree (decode i) in
+    if j =? i
+    then focus btctx_top (recover_bintree g' t) (decode j) = (g', t)
+    else if j =? (i * 2 + 1)
+         then match t with
+              | BT_nil => True
+              | BT_node x l r =>
+                  focus btctx_top (recover_bintree g' t) (decode j) = (btctx_left x r g', l)
+              end
+         else if j =? (i * 2 + 2)
+              then match t with
+                   | BT_nil => True
+                   | BT_node x l r =>
+                       focus btctx_top (recover_bintree g' t) (decode j) = (btctx_right x l g', r)
+                   end
+              else True.                                               
+  Admitted.
+
+
+   Lemma swap_subtree_left (tree : bintree A) i :
+    fromList (swap (toList tree) (i * 2 + 1) i) =
+      match focus btctx_top tree (decode i) with
+      | (_, BT_nil) => tree
+      | (_, BT_node x BT_nil _) => tree
+      | (g, BT_node x (BT_node xl ll lr) r) => recover_bintree g (BT_node xl (BT_node x ll lr) r)
+      end.
+  Admitted.
+  
+  Lemma swap_subtree_right (tree : bintree A) i :
+    fromList (swap (toList tree) (i * 2 + 2) i) =
+      match focus btctx_top tree (decode i) with
+      | (_, BT_nil) => tree
+      | (_, BT_node x _ BT_nil) => tree
+      | (g, BT_node x l (BT_node xr rl rr)) => recover_bintree g (BT_node xr l (BT_node x rl rr))
+      end.
+  Admitted.
+
+  Fixpoint btctx2idx (g : btctx A) : btidx :=
+    match g with
+    | btctx_top => []
+    | btctx_left _ _ g => btctx2idx g ++ [Dir_left]
+    | btctx_right _ _ g => btctx2idx g ++ [Dir_right]
+    end.
+
+  Lemma recover_option_subtree (g : btctx A) t :
+    option_subtree (btctx2idx g) (recover_bintree g t) = Some t.
+  Admitted.
+  
+  Lemma btctx2idx_focus tree i : let '(g, _) := focus btctx_top tree i in btctx2idx g = i.
+  Admitted.
+  
+  Theorem btctx_lookup (g : btctx A) t :
+    lookup (toList (recover_bintree g t)) (encode (btctx2idx g)) = option_root t.
+  Admitted.
+
+  Theorem recover_upd_root_repr_upd (t : bintree A) k g :
+    t <> BT_nil ->
+    toList (recover_bintree g (upd_root k t)) =
+    upd (toList (recover_bintree g t)) (encode (btctx2idx g)) k.
+  Admitted.
+
+End BinaryTreeZipper.
+
+Section ListAccessories.
+
+  Lemma list_extensionality {A : Type} (xs1 : list A) (xs2 : list A) :
+    xs1 = xs2 <-> (forall i, lookup xs1 i = lookup xs2 i).
+  Proof with discriminate || eauto.
+    revert xs1 xs2; cbn.
+    induction xs1 as [ | x1 xs1 IH]; intros [ | x2 xs2]; simpl in *; split; intros H_eq...
+    - pose (H_eq 0)...
+    - pose (H_eq 0)...
+    - rewrite H_eq...
+    - assert (H_x1_eq_x2 : x1 = x2) by exact (Some_inj (H_eq 0)); subst.
+      pose (proj2 (IH xs2) (fun i => H_eq (S i))); congruence.
+  Qed.
+
+  Lemma listExt_map {A : Type} {B : Type} (f : A -> B) (xs : list A) :
+    forall i, lookup (map f xs) i = option_map f (lookup xs i).
+  Proof. cbn; induction xs as [ | x xs IH]; intros [ | n']; simpl; (discriminate || eauto). Qed.
+
+  Lemma listExt_seq (start : nat) (len : nat) :
+    forall i,
+    match lookup (seq start len) i with
+    | None => i >= len
+    | Some x => x = start + i
+    end.
+  Proof with discriminate || eauto.
+    intros i.
+    destruct (nth_error (seq start len) i) as [x | ] eqn: H_obs.
+    - assert (i_lt_len : i < length (seq start len)).
+      { apply nth_error_Some. rewrite H_obs... }
+      rewrite (nth_error_nth' (seq start len) x i_lt_len) in H_obs.
+      apply Some_inj in H_obs; rewrite <- H_obs.
+      apply seq_nth; rewrite seq_length in i_lt_len...
+    - rewrite <- (seq_length len start); apply nth_error_None...
+  Qed.
+
+  Lemma firstn_nth_error {A : Type} (n : nat) (xs : list A)  :
+    forall i,
+    i < length xs ->
+    i < n ->
+    nth_error (firstn n xs) i = nth_error xs i.
+  Proof with discriminate || (try lia) || eauto.
+    revert xs; induction n as [ | n IH]; simpl...
+    intros [ | x xs] i H_lt1 H_lt2; simpl in *...
+    destruct i as [ | i']; simpl... apply IH...
+  Qed.
+
+  Lemma listExt_firstn {A : Type} (xs : list A) (n : nat) :
+    forall i,
+    match lookup (firstn n xs) i with
+    | None => i >= n \/ i >= length xs
+    | Some x => i < n /\ lookup xs i = Some x
+    end.
+  Proof with discriminate || (try lia) || eauto.
+    intros i.
+    destruct (nth_error (firstn n xs) i) as [x | ] eqn: H_obs.
+    - assert (i_lt_len : i < length (firstn n xs)).
+      { apply nth_error_Some. rewrite H_obs... }
+      pose (firstn_length n xs); split...
+      assert (i_lt_length_xs : i < length xs)...
+      rewrite <- H_obs; symmetry.
+      apply firstn_nth_error...
+    - assert (i_ge_len : i >= length (firstn n xs)).
+      { apply nth_error_None... }
+      rewrite (firstn_length n xs) in i_ge_len...
+  Qed.
+
+  Lemma listExt_skipn {A : Type} (xs : list A) (n : nat) :
+    forall i, lookup (skipn n xs) i = lookup xs (n + i).
+  Proof with eauto.
+    unfold lookup. revert n. induction xs as [ | x xs IH]; intros [ | n']; simpl... now destruct i.
+  Qed.
+
+  Lemma listExt_combine {A : Type} {B : Type} (xs : list A) (ys : list B) :
+    forall i,
+    match lookup (combine xs ys) i with
+    | None => i >= length xs \/ i >= length ys
+    | Some (x, y) => lookup xs i = Some x /\ lookup ys i = Some y
+    end.
+  Proof with discriminate || eauto.
+    set (len := min (length xs) (length ys)).
+    replace (combine xs ys) with (combine (firstn len xs) (firstn len ys)).
+    - assert (H_len : length (firstn len xs) = length (firstn len ys)).
+      { do 2 (rewrite firstn_length_le; [ | lia]); lia. }
+      intros i; cbn.
+      destruct (nth_error (combine (firstn len xs) (firstn len ys)) i) as [[x y] | ] eqn: H_obs.
+      + assert (H_i : i < length (combine (firstn len xs) (firstn len ys))).
+        { apply nth_error_Some; rewrite H_obs... }
+        assert (H1_i : i < length (firstn len xs)).
+        { pose (combine_length (firstn len xs) (firstn len ys)); lia. }
+        assert (H2_i : i < length (firstn len ys)).
+        { pose (combine_length (firstn len xs) (firstn len ys)); lia. }
+        assert (claim1 := listExt_firstn xs len i).
+        assert (claim2 := listExt_firstn ys len i).
+        rewrite (nth_error_nth' (firstn len xs) x H1_i) in claim1.
+        rewrite (nth_error_nth' (firstn len ys) y H2_i) in claim2.
+        rewrite (nth_error_nth' (combine (firstn len xs) (firstn len ys)) (x, y) H_i) in H_obs.
+        apply Some_inj in H_obs; rewrite (combine_nth (firstn len xs) (firstn len ys) i x y H_len) in H_obs.
+        assert (x_is : x = nth i (firstn len xs) x) by congruence.
+        assert (y_is : y = nth i (firstn len ys) y) by congruence.
+        rewrite x_is, y_is; now firstorder.
+      + enough (to_show : len <= i) by lia.
+        apply nth_error_None in H_obs.
+        rewrite combine_length in H_obs.
+        do 2 (rewrite firstn_length_le in H_obs; [ | lia]); lia.
+    - rewrite <- combine_firstn; apply firstn_all2; rewrite combine_length...
+  Qed.
+
+  Lemma listExt_add_indices {A : Type} (xs : list A) :
+    forall i, 
+    match lookup (add_indices xs) i with
+    | None => i >= length xs /\ lookup xs i = None
+    | Some (x, n) => i = n /\ lookup xs i = Some x
+    end.
+  Proof with discriminate || eauto.
+    intros i; unfold add_indices.
+    assert (claim1 := listExt_combine xs (seq 0 (length xs)) i).
+    destruct (nth_error (combine xs (seq 0 (length xs))) i) as [[x n] | ] eqn: H_obs.
+    - destruct claim1 as [H_obs_xs H_obs_seq]; split...
+      assert (claim2 := listExt_seq 0 (length xs) i).
+      rewrite H_obs_seq in claim2...
+    - rewrite seq_length in claim1.
+      rewrite nth_error_None; lia.
+  Qed.
+
+  Lemma listExt_swap {A : Type} (xs : list A) (i1 : nat) (i2 : nat) :
+    i1 < length xs ->
+    i2 < length xs ->
+    forall i,
+    match lookup (swap xs i1 i2) i with
+    | None => i >= length xs
+    | Some val =>
+      Some val =
+      if Nat.eq_dec i i1 then lookup xs i2 else
+      if Nat.eq_dec i i2 then lookup xs i1 else
+      lookup xs i
+    end.
+  Proof with discriminate || eauto.
+    intros H_i1 H_i2.
+    assert (H_lookup_i1 := proj2 (nth_error_Some xs i1) H_i1).
+    assert (H_lookup_i2 := proj2 (nth_error_Some xs i2) H_i2).
+    intros i; cbn; unfold swap.
+    assert (claim1 := listExt_map (uncurry (swap_aux xs i1 i2)) (add_indices xs) i).
+    rewrite claim1; unfold option_map.
+    assert (claim2 := listExt_add_indices xs i).
+    destruct (nth_error (add_indices xs) i) as [[x n] | ] eqn: H_obs_add_indices.
+    - simpl; unfold swap_aux, lookup.
+      destruct claim2 as [H_EQ H_obs_xs]; subst n.
+      destruct (Nat.eq_dec i i1) as [H_yes1 | H_no1].
+      { subst i. symmetry; apply nth_error_nth'... } 
+      destruct (Nat.eq_dec i i2) as [H_yes2 | H_no2].
+      { subst i. symmetry; apply nth_error_nth'... }
+      symmetry...
+    - exact (proj1 claim2).
+  Qed.
+
+  Lemma add_indices_length {A : Type} (xs : list A) :
+    length (add_indices xs) = length xs.
+  Proof with lia || discriminate || eauto.
+    transitivity (length (map snd (add_indices xs))).
+    { symmetry. apply map_length. }
+    transitivity (length (seq 0 (length xs))).
+    { apply f_equal. apply list_extensionality.
+      intros i.
+      rewrite (listExt_map snd (add_indices xs) i).
+      assert (claim1 := listExt_add_indices xs i).
+      assert (claim2 := listExt_seq 0 (length xs) i).
+      destruct (lookup (add_indices xs) i) as [[x n] | ] eqn: H_obs.
+      - destruct claim1 as [H_eq H_obs_xs].
+        subst n. simpl. symmetry.
+        destruct (lookup (seq 0 (length xs)) i) as [i_ | ]; subst...
+        apply isSome_intro, nth_error_Some in H_obs_xs...
+      - destruct claim1 as [H_eq H_obs_xs].
+        simpl. symmetry. apply nth_error_None. rewrite seq_length...
+    }
+    rewrite seq_length...
+  Qed.
+
+  Lemma listExt_upd {A : Type} (xs : list A) (i1 : nat) (x1 : A) :
+    i1 < length xs ->
+    forall i,
+    match lookup (upd xs i1 x1) i with
+    | None => i >= length xs
+    | Some val => Some val = if Nat.eq_dec i i1 then Some x1 else lookup xs i
+    end.
+  Proof with discriminate || eauto.
+    intros H_i1.
+    assert (H_lookup_i1 := proj2 (nth_error_Some xs i1) H_i1).
+    intros i; cbn; unfold upd.
+    assert (claim1 := listExt_map (fun '(x, i0) => if eq_dec i0 i1 then x1 else x) (add_indices xs) i).
+    rewrite claim1; unfold option_map.
+    assert (claim2 := listExt_add_indices xs i).
+    destruct (nth_error (add_indices xs) i) as [[x n] | ] eqn: H_obs_add_indices.
+    - destruct claim2 as [H_eq1 H_eq2]; subst n.
+      destruct (Nat.eq_dec i i1) as [H_yes1 | H_no1]...
+    - exact (proj1 claim2).
+  Qed.
+
+  Theorem upd_spec {A : Type} (xs : list A) i x :
+    upd xs i x = if Nat.ltb i (length xs) then firstn i xs ++ [x] ++ skipn (i + 1) xs else xs.
+  Proof with lia || eauto.
+    rename i into i0, x into x0.
+    destruct (Nat.ltb i0 (length xs)) eqn: H_range.
+    - apply Nat.ltb_lt in H_range.
+      assert (claim1 := listExt_upd xs i0 x0 H_range).
+      transitivity (firstn i0 xs ++ (firstn 1 (x0 :: skipn (S i0) xs) ++ skipn 1 (x0 :: skipn (S i0) xs))).
+      2: rewrite firstn_skipn; replace (i0 + 1) with (S i0)...
+      transitivity (firstn i0 (upd xs i0 x0) ++ skipn i0 (upd xs i0 x0)).
+      1: symmetry; apply firstn_skipn.
+      f_equal.
+      { apply list_extensionality.
+        intros i. specialize (claim1 i).
+        assert (claim2 := listExt_firstn (upd xs i0 x0) i0 i).
+        destruct (lookup (firstn i0 (upd xs i0 x0)) i) as [x | ] eqn: H_obs.
+        - destruct claim2 as [H_i_lt_i0 H_x].
+          rewrite H_x in claim1.
+          destruct (Nat.eq_dec i i0) as [H_yes1 | H_no1]...
+          rewrite claim1. symmetry. apply firstn_nth_error...
+        - symmetry. apply nth_error_None. rewrite firstn_length.
+          enough (to_show : i >= i0 \/ i >= length xs)...
+          unfold upd in claim2. rewrite map_length in claim2.
+          rewrite add_indices_length in claim2...
+      }
+      { apply list_extensionality.
+        intros i.
+        rewrite listExt_skipn.
+        destruct i as [ | i'].
+        - rewrite Nat.add_0_r. simpl.
+          specialize (claim1 i0).
+          destruct (lookup (upd xs i0 x0) i0) as [x | ]...
+          destruct (Nat.eq_dec i0 i0)...
+        - rewrite firstn_skipn.
+          replace ((S i')) with (1 + i') at 2 by lia.
+          rewrite <- listExt_skipn with (xs0 := (x0 :: skipn (S i0) xs)).
+          set (xs_suffix := skipn (S i0) xs).
+          simpl. unfold xs_suffix. specialize (claim1 (i0 + S i')).
+          destruct (lookup (upd xs i0 x0) (i0 + S i')) as [x | ].
+          + destruct (Nat.eq_dec (i0 + S i') i0) as [H_yes1 | H_no1]...
+            rewrite claim1. replace (i0 + S i') with (S i0 + i')...
+            symmetry. apply listExt_skipn.
+          + symmetry. apply nth_error_None.
+            rewrite skipn_length...
+      }
+    - apply Nat.ltb_nlt in H_range.
+      unfold upd. apply list_extensionality. intros i.
+      rewrite (listExt_map (fun '(x, i1) => if eq_dec i1 i0 then x0 else x) (add_indices xs) i).
+      assert (claim1 := listExt_add_indices xs i).
+      destruct (lookup (add_indices xs) i) as [[x n] | ] eqn: H_obs.
+      + destruct claim1 as [H_eq H_obs_xs]; subst.
+        simpl. destruct (Nat.eq_dec n i0); [subst n | ]...
+        apply isSome_intro, nth_error_Some in H_obs_xs...
+      + simpl. now symmetry.
+  Qed.
+
+  Lemma upd_length {A : Type} (xs : list A) i0 x0 : length (upd xs i0 x0) = length xs.
+  Proof. unfold upd. rewrite map_length. apply add_indices_length. Qed.
+
+End ListAccessories.
+
+(*
+Module NEO.
+
+  Section BinaryTreeAccessories.
+
+  Context {A : Type}.
+
+  Definition toListAux root := map (fun i => @option_rect (bintree A) (fun _ => option A) option_root None (option_subtree (decode i) root)) (seq 0 ((2 ^ rank root) - 1)).
+
+  Definition toList root := flat_map option2list (toListAux root).
+
+  Definition insertInit (x : A) (t : bintree A) :=
+    match t with
+    | BT_nil => Some (BT_node x BT_nil BT_nil)
+    | BT_node x l r => None
+    end.
+
+  Definition insertStep d acc t : option (bintree A) :=
+    match t with
+    | BT_nil => None
+    | BT_node x l r =>
+      match d with
+      | Dir_left => option_map (fun l' => BT_node x l' r) (acc l)
+      | Dir_right => option_map (fun r' => BT_node x l r') (acc r)
+      end
+    end.
+
+  Definition insertAt (x : A) : btidx -> bintree A -> option (bintree A) := fold_right insertStep (insertInit x).
+
+  Definition insertable (root : bintree A) i := subtree_nat root i = Some BT_nil.
+
+  Definition fromListStep root := fun '(x, i) => @option_rect (bintree A) (fun _ => bintree A) id root (insertAt x (decode i) root).
+
+  Definition fromList xs := fold_left fromListStep (add_indices xs) BT_nil.
+
+  Definition isComplete root := Forall isSome (firstn (btsize root) (toListAux root)) /\ Forall isNone (skipn (btsize root) (toListAux root)).
+
+  End BinaryTreeAccessories.
+
+End NEO.
+*)
